DS/Tree.v
@@ -1,0 +1,256 @@
+Add Rec LoadPath "/home/zeimer/Code/Coq".
+
+Require Export LinDec.
+Require Export RCCBase.
+
+Inductive Tree (A : Type) : Type :=
+    | E : Tree A
+    | T : A -> list (Tree A) -> Tree A.
+
+Arguments E [A].
+Arguments T [A] _ _.
+
+Fixpoint Tree_rect'
+  (A : Type) (P : Tree A -> Type) (Q : list (Tree A) -> Type)
+  (HE : P E)
+  (Hnil : Q [])
+  (Hcons : forall (h : Tree A) (t : list (Tree A)), P h -> Q t -> Q (h :: t))
+  (Htrans : forall (x : A) (l : list (Tree A)), Q l -> P (T x l))
+  (t : Tree A) : P t.
+Proof.
+  destruct t.
+    assumption.
+    apply Htrans. induction l as [| h t].
+      assumption.
+      apply Hcons.
+        eapply Tree_rect'; eauto.
+        assumption.
+Defined.
+
+Theorem Tree_ind_proper
+  (A : Type) (P : Tree A -> Prop)
+  (HE : P E)
+  (HT : forall (x : A) (l : list (Tree A)), Forall P l -> P (T x l))
+  (t : Tree A) : P t.
+Proof.
+  induction t using Tree_rect' with (Q := Forall P); auto.
+Qed.
+
+Theorem Tree_ind_proper'
+  (A : Type) (P : Tree A -> Prop)
+  (HE : P E)
+  (Hnil : forall x : A, P (T x []))
+  (HT : forall (x : A) (t : Tree A) (l : list (Tree A)),
+    P t -> Forall P l -> P (T x (t :: l)))
+  (t : Tree A) : P t.
+Proof.
+  induction t using Tree_ind_proper; auto.
+  destruct l.
+    apply Hnil.
+    apply HT; inv H.
+Qed.
+
+Lemma Tree_ind_proper2
+  (A : Type) (P : Tree A -> Prop)
+  (HE : P E)
+  (Hnil : forall x : A, P (T x []))
+  (HT : forall (x : A) (t : Tree A) (ts : list (Tree A)),
+    P t -> P (T x ts) -> P (T x (t :: ts)))
+  (t : Tree A) : P t.
+Proof.
+  induction t using Tree_ind_proper.
+    apply HE.
+    induction H.
+      apply Hnil.
+      apply HT; assumption.
+Qed.
+
+Inductive elem {A : Type} (x : A) : Tree A -> Prop :=
+    | elem0 : forall l : list (Tree A), elem x (T x l)
+    | elem1 : forall (a : A) (l : list (Tree A)),
+        Exists (fun t => elem x t) l -> elem x (T a l).
+
+Inductive elem' {A : Type} (x : A) : Tree A -> Prop :=
+    | elem0' : forall l : list (Tree A), elem' x (T x l)
+    | elem1' :
+        forall (a : A) (t : Tree A) (ts : list (Tree A)),
+          elem' x t -> elem' x (T a (t :: ts))
+    | elem2' :
+        forall (a : A) (t : Tree A) (ts : list (Tree A)),
+          elem' x (T a ts) -> elem' x (T a (t :: ts)). 
+
+Inductive isHeap {A : LinDec} : Tree A -> Prop :=
+    | isHeap_E : isHeap E
+    | isHeap_T :
+        forall (v : A) (l : list (Tree A)),
+          Forall (fun t : Tree A => forall x : A, elem x t -> v ≤ x) l ->
+          Forall (fun t : Tree A => isHeap t) l ->
+            isHeap (T v l).
+
+(*Lemma isHeap_inv :
+  forall (A : LinDec) (x : A) (l : list (Tree A)),
+    isHeap (T x l) -> Forall isHeap l.
+Proof.
+  intros. inv H.
+Qed.
+
+Lemma isHeap_inv' :
+  forall (A : LinDec) (v : A) (l : list (Tree A)),
+    isHeap (T v l) ->
+      Forall (fun t : Tree A => forall x : A, elem x t -> v ≤ x) l.
+Proof.
+  intros. inv H.
+Qed.*)
+
+Hint Constructors elem isHeap.
+
+Require Import HSLib.Control.Functor.
+
+Fixpoint fmap_Tree
+  {A B : Type} (f : A -> B) (t : Tree A) : Tree B :=
+match t with
+    | E => E
+    | T x l => T (f x) (map (fmap_Tree f) l)
+end.
+
+Ltac Tree_ind :=
+repeat match goal with
+    | |- forall t' : Tree _, _ =>
+        let x := fresh "x" in
+        let t := fresh "t" in
+        let ts := fresh "ts" in
+        let IHt := fresh "IHt" in
+        let IHts := fresh "IHts" in
+          induction t' as [| x | x t ts IHt IHts] using Tree_ind_proper2;
+          cbn in *; try reflexivity; f_equal; rewrite ?IHt; auto;
+          try (inv IHts; fail)
+    | |- forall _, _ => intro
+end.
+
+Instance Functor_Tree : Functor Tree :=
+{
+    fmap := @fmap_Tree
+}.
+Proof.
+  all: intros; ext t.
+    destruct t as [| x t] using Tree_ind_proper; cbn.
+      reflexivity.
+      induction H; cbn.
+        reflexivity.
+        rewrite !id_eq in *. f_equal. inv IHForall.
+    destruct t as [| x t] using Tree_ind_proper; cbn.
+      reflexivity.
+      induction H; cbn.
+        reflexivity.
+        f_equal. inv IHForall. rewrite H2. f_equal. assumption.
+Restart.
+  all: intros; ext t.
+    induction t as [| x | x t ts] using Tree_ind_proper2;
+    cbn in *; rewrite !id_eq in *; try reflexivity.
+      rewrite IHt. inv IHt0.
+    induction t as [| x | x t ts] using Tree_ind_proper2;
+    cbn in *; try reflexivity.
+      rewrite IHt. inv IHt0.
+Restart.
+  all: intros; ext t; gen t; Tree_ind.
+
+(*Hint Extern 1 =>
+match goal with
+    | |- context [id _] => rewrite ?id_eq; try congruence
+end.*)
+
+    rewrite !id_eq. inv IHts.
+Defined.
+
+Fixpoint size {A : Type} (t : Tree A) : nat :=
+match t with
+    | E => 0
+    | T _ ts => 1 + fold_right (fun h t => size h + t) 0 ts
+end.
+
+Lemma fmap_size :
+  forall (A B : Type) (f : A -> B) (t : Tree A),
+    size (fmap_Tree f t) = size t.
+Proof.
+  Tree_ind.
+Qed.
+
+Hint Constructors elem'.
+
+Hint Extern 0 =>
+match goal with
+    | H : elem' _ E |- _ => inv H
+end.
+
+Lemma fmap_elem' :
+  forall (A B : Type) (f : A -> B) (t : Tree A) (x : A),
+    elem' x t -> elem' (f x) (fmap_Tree f t).
+Proof.
+  induction 1; cbn; auto.
+Qed.
+
+(*Lemma fmap_elem :
+  forall (A B : Type) (f : A -> B) (t : Tree A) (x : A),
+    elem x t -> elem (f x) (fmap_Tree f t).
+Proof.
+  induction 1; cbn; auto.
+    induction H. cbn.
+Qed.*)
+
+Require Import HSLib.Control.Foldable.
+
+Print Foldable.
+
+Fixpoint foldMap_Tree
+  {A : Type} {M : Monoid} (f : A -> M) (t : Tree A) : M :=
+match t with
+    | E => neutr
+    | T x l => op (f x)
+                  (fold_right (fun h t => op (foldMap_Tree f h) t) neutr l)
+        (*let aux := fix aux (l : list (Tree A)) : M :=
+        match l with
+            | [] => neutr
+            | t :: ts => op (foldMap_Tree f t) (aux ts)
+        end
+        in op (f x) (aux l)*)
+end.
+
+Instance Foldable_Tree : Foldable Tree :=
+{
+    foldMap := @foldMap_Tree;
+}.
+Proof.
+  intros. ext t. gen t.
+  destruct t as [| x l].
+    unfold compose; cbn. rewrite H. reflexivity.
+    induction l as [| t ts].
+      unfold compose; cbn. rewrite !id_right. reflexivity.
+      unfold compose in *; cbn in *. rewrite H0 in *.
+        rewrite H0 in *. inv IHts.
+Restart.
+  intros. ext t. gen t.
+  induction t using Tree_ind_proper.
+    unfold compose; cbn. rewrite H. reflexivity.
+    induction H1.
+      unfold compose; cbn. rewrite !id_right. reflexivity.
+      unfold compose in *; cbn in *.
+        rewrite <- ?op_assoc in *. rewrite !H0. f_equal.
+Restart.
+  intros. ext t. gen t. fix 1.
+  destruct t as [| x [| t ts]].
+    unfold compose; cbn. rewrite H. reflexivity.
+    unfold compose; cbn. rewrite !id_right. reflexivity.
+Restart.
+  intros. ext t. gen t.
+  apply (@Tree_rect' _ _ (fun l =>
+      fold_right (fun t ts => op (foldMap_Tree (f .> g) t) ts) neutr l =
+      fold_right (fun t ts => op (g (foldMap_Tree f t)) ts) neutr l)).
+    unfold compose; cbn. rewrite H. reflexivity.
+    cbn. reflexivity.
+    intros. cbn. rewrite H1, H2. reflexivity.
+    intros. unfold compose in *. cbn in *. rewrite ?H1, H0.
+      f_equal. clear H1. induction l as [| h t]; cbn.
+        rewrite H. reflexivity.
+        rewrite H0.
+        rewrite IHt. reflexivity.
+Defined.
